<?xml version="1.0" encoding="UTF-8" ?>
<rdf:RDF
   xml:base="http://powl.sf.net/WCMS/Layout/0.1#"
   xmlns:rdf="http://www.w3.org/1999/02/22-rdf-syntax-ns#"
   xmlns:rdfs="http://www.w3.org/2000/01/rdf-schema#"
   xmlns:ns1="http://www.w3.org/2002/07/owl#">

<rdfs:Class rdf:ID="ClassTemplate">
   <rdfs:comment>The class for class templates.</rdfs:comment>
   <rdfs:subClassOf rdf:resource="#Template"/>
</rdfs:Class>

<rdfs:Class rdf:ID="OverviewTemplate">
   <rdfs:comment>The class for overview templates. </rdfs:comment>
   <rdfs:subClassOf rdf:resource="#Template"/>
</rdfs:Class>

<rdfs:Class rdf:ID="PropertyTemplate">
   <rdfs:comment>The class for property templates.</rdfs:comment>
   <rdfs:subClassOf rdf:resource="#Template"/>
</rdfs:Class>

<ns1:Class rdf:ID="Template">
   <rdfs:comment>The class of templates. It provides the properties templateDefinition and templateResource. These are used to attach templates to properties and classes of the content ontology.</rdfs:comment>
</ns1:Class>

<ns1:DatatypeProperty rdf:ID="templateDefinition">
   <rdfs:comment>This property contains the template data for properties, classes or overview pages.</rdfs:comment>
   <rdfs:domain rdf:resource="#Template"/>
   <rdfs:range rdf:resource="http://www.w3.org/2001/XMLSchema#string"/>
</ns1:DatatypeProperty>

<ns1:DatatypeProperty rdf:ID="templateResource">
   <rdfs:comment>This property defines the resource (a class or a property) for a template. The given resource will be rendered with its templateDefinition on the website.</rdfs:comment>
   <rdfs:domain rdf:resource="#Template"/>
   <rdfs:range rdf:resource="http://www.w3.org/2001/XMLSchema#string"/>
</ns1:DatatypeProperty>

<rdf:Description rdf:about="http://powl.sf.net/WCMS/Layout/0.1">
   <rdfs:comment>The layout ontology contains classes and properties representing the layout for the website. Since all content ist stored in property values attached to class instances, the layout information is related to these properties and classes. Therefore this ontology defines classes for class and property templates.</rdfs:comment>
</rdf:Description>

</rdf:RDF>